JaIrisSoundness.v
@@ -1815,14 +1815,12 @@ Proof.
   intros env h gamma_match_env.
   intros h_satisfies_s confs hn res_ex res new_env h_satisfies_p let_eval.
 
-  set (let_evaluation := LetEvaluationEx h class x e1 e2 confs hn res_ex res env CC let_eval).
-  destruct let_evaluation as [(confs_e1 & e1_ex & e1_res & ex_eq & e1_eval) |
-                              (confs_e1 & confs_e2 & h' & e1_res & e1_eval & e2_eval)].
-  + rewrite ex_eq in e1_eval.
-    destruct (IH_e1 env h gamma_match_env h_satisfies_s confs_e1 hn (Some e1_ex) e1_res h_satisfies_p e1_eval)
-      as (false_eq & _).
-    discriminate false_eq.
-  + apply LetRuleE2Soundness with (h' := h') (x := x) (e1_res := e1_res) (e2 := e2)
+  set (let_evaluation := LetEvaluation h class x e1 e2 confs hn res res_ex env CC let_eval).
+  destruct let_evaluation as
+    [(confs_e1 & confs_e2 & h' & e1_res & e1_eval & e2_eval) | (confs_e1 & h' & e1_res & e1_ex & e1_eval)].
+  + assert (asdf := IH_e2 env h gamma_match_env h_satisfies_s).
+    simpl in asdf.
+    apply LetRuleE2Soundness with (h' := h') (x := x) (e1_res := e1_res) (e2 := e2)
       (confs_e2 := confs_e2) (class := class) (ex := ex) (v := v) (q := q).
     ++ admit. (* e1_res type *)
     ++ assumption.
@@ -1833,7 +1831,10 @@ Proof.
        +++ apply EvaluationPreservesGammaMatching with (h := h) (e := (JFIExprSubstituteEnv env e1))
              (confs := confs_e1) (ex := None) (res := e1_res) (CC := CC); assumption.
        +++ apply EvaluationPreservesPersistentTerms with (h := h) (e := (JFIExprSubstituteEnv env e1))
-          (confs := confs_e1) (ex := None) (res := e1_res); assumption.
+             (confs := confs_e1) (ex := None) (res := e1_res); assumption.
+  + assert (some_is_none := IH_e1 env h gamma_match_env h_satisfies_s confs_e1 h' (Some e1_ex) e1_res h_satisfies_p e1_eval).
+    fold JFIHeapSatisfiesInEnv in some_is_none.
+    discriminate (proj1 some_is_none).
 Admitted.
 Hint Resolve HTLetRuleSoundness : core.
 
